specs/Spec.Stream.fsti
@@ -27,10 +27,22 @@ unfold let avail_out_unchange (s0 s1: stream_state) = U32.v s0.[2] == U32.v s1.[
 unfold let total_out_unchange (s0 s1: stream_state) = U32.v s0.[3] == U32.v s1.[3]
 unfold let adler_unchange (s0 s1: stream_state) = U32.v s0.[4] == U32.v s1.[4]
 
-unfold let next_in_valid
+private let adler_valid
   (h: HS.mem)
-  (s: B.lbuffer U32.t 5)
-  (next_in: B.pointer (B.buffer U8.t)) =
+  (s: stream_state_t)
+  (wrap: wrap_t)
+  (block_data: Seq.seq U8.t) =
+  let s' = B.as_seq h s in
+  let len = Seq.length block_data in
+  (I32.v wrap == 1 ==>
+    Adler32.adler32_matched #len block_data (adler s')) /\
+  (I32.v wrap == 2 ==>
+    CRC32.crc32_matched len block_data (adler s') true)
+
+private unfold let next_in_valid
+  (h: HS.mem)
+  (s: stream_state_t)
+  (next_in: io_buffer) =
   let next_in' = B.get h next_in 0 in
   B.frameOf next_in == B.frameOf s /\
   B.frameOf next_in' == B.frameOf s /\
@@ -38,10 +50,10 @@ unfold let next_in_valid
   B.disjoint next_in s /\ B.disjoint next_in' s /\ B.disjoint next_in next_in' /\
   B.length next_in' == avail_in (B.as_seq h s)
 
-unfold let next_out_valid
+private unfold let next_out_valid
   (h: HS.mem)
-  (s: B.lbuffer U32.t 5)
-  (next_out: B.pointer (B.buffer U8.t)) =
+  (s: stream_state_t)
+  (next_out: io_buffer) =
   let next_out' = B.get h next_out 0 in
   B.frameOf next_out == B.frameOf s /\
   B.frameOf next_out' == B.frameOf s /\
@@ -49,27 +61,29 @@ unfold let next_out_valid
   B.disjoint next_out s /\ B.disjoint next_out' s /\ B.disjoint next_out next_out' /\
   B.length next_out' == avail_out (B.as_seq h s)
 
-unfold let adler_valid
+let istream_valid
   (h: HS.mem)
   (s: stream_state_t)
-  (wrap: I32.t)
-  (uncompressed: Seq.seq U8.t) =
-  let s' = B.as_seq h s in
-  let len = Seq.length uncompressed in
-  (I32.v wrap == 1 ==>
-    Adler32.adler32_matched #len uncompressed (adler s')) /\
-  ((CFlags.gzip == true /\ I32.v wrap == 2) ==>
-    CRC32.crc32_matched len uncompressed (adler s') true)
-
+  (next_in: io_buffer)
+  (wrap: wrap_t)
+  (block_data: Seq.seq U8.t) =
+  B.live h s /\ next_in_valid h s next_in /\ adler_valid h s wrap block_data
+  
+let ostream_valid
+  (h: HS.mem)
+  (s: stream_state_t)
+  (next_out: B.pointer (B.buffer U8.t))
+  (wrap: wrap_t)
+  (block_data: Seq.seq U8.t) =
+  B.live h s /\ next_out_valid h s next_out /\ adler_valid h s wrap block_data
+  
 let stream_valid
   (h: HS.mem)
   (s: stream_state_t)
   (next_in: B.pointer (B.buffer U8.t))
   (next_out: B.pointer (B.buffer U8.t))
-  (wrap: I32.t)
-  (uncompressed: Seq.seq U8.t) =
-  let s' = B.as_seq h s in
-  let len = Seq.length uncompressed in
+  (wrap: wrap_t)
+  (block_data: Seq.seq U8.t) =
   let next_out' = B.get h next_out 0 in
   let next_in' = B.get h next_in 0 in
   B.live h s /\
@@ -79,20 +93,20 @@ let stream_valid
   B.disjoint next_in' next_out' /\
 
   next_in_valid h s next_in /\ next_out_valid h s next_out /\
-  adler_valid h s wrap uncompressed
+  adler_valid h s wrap block_data
 
 private unfold let read_buf_size(h: HS.mem) (s: stream_state_t) (size: U32.t) =
   let s' = B.as_seq h s in
   if U32.v size > avail_in s' then avail_in s' else U32.v size
 
-let read_buf_pre
+unfold let read_buf_pre
   (h: HS.mem)
   (s: stream_state_t)
-  (uncompressed: Seq.seq U8.t)
+  (block_data: Seq.seq U8.t)
   (next_in: B.pointer (B.buffer U8.t))
   (buf: B.buffer U8.t)
   (size: U32.t)
-  (wrap: I32.t) =
+  (wrap: wrap_t) =
   let len = read_buf_size h s size in
   len > 0 /\
   B.live h s /\ ~(B.g_is_null s) /\
@@ -100,33 +114,37 @@ let read_buf_pre
   HS.disjoint (B.frameOf s) (B.frameOf buf) /\
   B.length buf == U32.v size /\
   next_in_valid h s next_in /\
-  adler_valid h s wrap uncompressed
+  adler_valid h s wrap block_data
 
 let read_buf_post
   (h0: HS.mem)
   (res: (U32.t & Ghost.erased (B.buffer U8.t)))
   (h1: HS.mem)
   (s: stream_state_t)
-  (uncompressed: Seq.seq U8.t)
+  (block_data: Seq.seq U8.t)
   (next_in: B.pointer (B.buffer U8.t))
   (buf: B.buffer U8.t)
   (size: U32.t)
-  (wrap: I32.t) =
+  (wrap: wrap_t) =
   let (len', read) = res in
   let next_in0 = B.get h0 next_in 0 in
   let next_in1 = B.get h1 next_in 0 in
+  let b1 = B.as_seq h1 buf in
   let s0 = B.as_seq h0 s in
   let s1 = B.as_seq h1 s in
   let len = read_buf_size h0 s size in
+  read_buf_pre h0 s block_data next_in buf size wrap /\
   len == U32.v len' /\
   B.modifies (
     B.loc_buffer s `B.loc_union`
     B.loc_buffer next_in `B.loc_union`
     B.loc_buffer buf) h0 h1 /\
   U32.v len' <= B.length next_in0 /\
+  Ghost.reveal read == B.gsub next_in0 0ul len' /\
   Seq.equal (B.as_seq h1 read) (B.as_seq h0 (B.gsub next_in0 0ul len')) /\
+  Seq.equal (B.as_seq h1 read) (B.as_seq h1 (B.gsub buf 0ul len')) /\
+  next_in1 == B.gsub next_in0 len' (U32.uint_to_t ((avail_in s0) - len)) /\
   avail_in s0 - len == avail_in s1 /\
   next_in_valid h1 s next_in /\
-  adler_valid h1 s wrap (Seq.append uncompressed (B.as_seq h1 read)) /\
-  avail_out_unchange s0 s1 /\
-  total_out_unchange s0 s1
+  adler_valid h1 s wrap (Seq.append block_data (B.as_seq h1 read)) /\
+  avail_out_unchange s0 s1 /\ total_out_unchange s0 s1
