code/Yazi.Stream.State.fst
@@ -1,0 +1,58 @@
+module Yazi.Stream.State
+
+module B = LowStar.Buffer
+module LB = Lib.Buffer
+module S = Spec.Stream
+module ST = FStar.HyperStack.ST
+module U32 = FStar.UInt32
+
+open LowStar.BufferOps
+open Yazi.Stream.Types
+
+inline_for_extraction
+let get_avail_in (s: stream_state_t): ST.Stack U32.t
+  (requires fun h -> B.live h s)
+  (ensures fun h0 res h1 ->
+    B.modifies B.loc_none h0 h1 /\ U32.v res == S.avail_in (B.as_seq h0 s)) =
+  s.(0ul)
+
+inline_for_extraction
+let set_avail_in (s: stream_state_t) (a: U32.t): ST.Stack unit
+  (requires fun h -> B.live h s)
+  (ensures fun h0 _ h1 ->
+    B.modifies (B.loc_buffer s) h0 h1 /\
+    U32.v a == S.avail_in (B.as_seq h1 s) /\
+    LB.unchange_except h0 h1 s 0) =
+  s.(0ul) <- a
+
+inline_for_extraction
+let get_total_in (s: stream_state_t): ST.Stack U32.t
+  (requires fun h -> B.live h s)
+  (ensures fun h0 res h1 ->
+    B.modifies B.loc_none h0 h1 /\ U32.v res == S.total_in (B.as_seq h0 s)) =
+  s.(1ul)
+
+inline_for_extraction
+let set_total_in (s: stream_state_t) (a: U32.t): ST.Stack unit
+  (requires fun h -> B.live h s)
+  (ensures fun h0 _ h1 ->
+    B.modifies (B.loc_buffer s) h0 h1 /\
+    U32.v a == S.total_in (B.as_seq h1 s) /\
+    LB.unchange_except h0 h1 s 1) =
+  s.(1ul) <- a
+
+inline_for_extraction
+let get_adler (s: stream_state_t): ST.Stack U32.t
+  (requires fun h -> B.live h s)
+  (ensures fun h0 res h1 ->
+    B.modifies B.loc_none h0 h1 /\ U32.v res == U32.v (S.adler (B.as_seq h0 s))) =
+  s.(4ul)
+
+inline_for_extraction
+let set_adler (s: stream_state_t) (a: U32.t): ST.Stack unit
+  (requires fun h -> B.live h s)
+  (ensures fun h0 _ h1 ->
+    B.modifies (B.loc_buffer s) h0 h1 /\
+    U32.v a == U32.v (S.adler (B.as_seq h1 s)) /\
+    LB.unchange_except h0 h1 s 4) =
+  s.(4ul) <- a
