code/Yazi.Stream.Types.fsti
@@ -1,6 +1,16 @@
 module Yazi.Stream.Types
 
 module B = LowStar.Buffer
+module CFlags = Yazi.CFlags
+module I32 = FStar.Int32
 module U32 = FStar.UInt32
+module U8 = FStar.UInt8
 
 type stream_state_t = B.lbuffer U32.t 5
+
+type wrap_t = w: I32.t{
+  let w' = I32.v w in
+  w' == 0 \/ w' == 1 \/ (CFlags.gzip == true /\ w' == 2)
+}
+
+type io_buffer = B.pointer (B.buffer U8.t)
